theories/cap_lang.v
@@ -209,7 +209,23 @@ Section opsem.
     match i with
     | Fail => Some (Failed, φ)
     | Halt => Some (Halted, φ)
+    (* NOTE: if IE, just put the capability as it is in the register *)
     | Jmp r =>
+        wr ← (reg φ) !! r;
+        (* Note: allow jumping to integers, sealing ranges etc; machine will crash later *)
+        let φ' := (update_reg φ PC (updatePcPerm wr)) in
+        Some (NextI, φ')
+    | Jnz r1 r2 =>
+      wr2 ← (reg φ) !! r2;
+      wr1 ← (reg φ) !! r1;
+      if nonZero wr2
+      then
+        (* Note: allow jumping to integers, sealing ranges etc; machine will crash later *)
+        let φ' := (update_reg φ PC (updatePcPerm wr1)) in
+        Some (NextI, φ')
+      else updatePC φ
+    (* NOTE: jmp fails if not an IE *)
+    | JmpIEpair r =>
       wr ← (reg φ) !! r;
       match wr with
       | WCap IE b e a =>
@@ -220,31 +236,9 @@ Section opsem.
           let φ' := (update_reg (update_reg φ PC wpc) idc widc) in
           Some (NextI, φ')
         else None
-      | _ =>
-          (* Note: allow jumping to integers, sealing ranges etc; machine will crash later *)
-          let φ' := (update_reg φ PC (updatePcPerm wr)) in
-          Some (NextI, φ')
+      | _ => None
       end
-    | Jnz r1 r2 =>
-      wr2 ← (reg φ) !! r2;
-      wr1 ← (reg φ) !! r1;
-      if nonZero wr2
-      then
-        match wr1 with
-        | WCap IE b e a =>
-            if withinBounds b e a && withinBounds b e (a^+1)%a
-            then
-              wpc ← (mem φ) !! a;
-              widc ← (mem φ) !! (a^+1)%a;
-              let φ' := (update_reg (update_reg φ PC wpc) idc widc) in
-              Some (NextI, φ')
-            else None
-        | _ =>
-            (* Note: allow jumping to integers, sealing ranges etc; machine will crash later *)
-            let φ' := (update_reg φ PC (updatePcPerm wr1)) in
-            Some (NextI, φ')
-        end
-      else updatePC φ
+    (*   else updatePC φ *)
     | Load dst src =>
       wsrc ← (reg φ) !! src;
       match wsrc with
