theories/ftlr/JmpIEpair.v
@@ -1,0 +1,551 @@
+From iris.proofmode Require Import proofmode.
+From iris.program_logic Require Import weakestpre adequacy lifting.
+From stdpp Require Import base.
+From cap_machine Require Export logrel register_tactics.
+From cap_machine.ftlr Require Import ftlr_base.
+From cap_machine.rules Require Import rules_JmpIEpair.
+
+Section fundamental.
+  Context {Σ:gFunctors} {memg:memG Σ} {regg:regG Σ} {sealsg: sealStoreG Σ}
+          {nainv: logrel_na_invs Σ}
+          `{MachineParameters}.
+
+  Notation D := ((leibnizO Word) -n> iPropO Σ).
+  Notation R := ((leibnizO Reg) -n> iPropO Σ).
+  Implicit Types w : (leibnizO Word).
+  Implicit Types interp : (D).
+
+  (* The first part is common with Jnz. The argument =cond=
+     expresses the pure conditions specific to the kind of jump.
+   *)
+
+  (* Mask after the jump, depending on the address of the pc and the address
+   of a *)
+  Definition allow_jmp_mask (pc_a a a' : Addr) : coPset
+    :=
+    if decide (pc_a = a)
+    then (⊤ ∖ ↑logN.@pc_a ∖ ↑logN.@a')
+    else
+      if decide (pc_a = a')
+      then (⊤ ∖ ↑logN.@pc_a ∖ ↑logN.@a)
+      else (⊤ ∖ ↑logN.@pc_a ∖ ↑logN.@a ∖ ↑logN.@a').
+
+  Definition allow_jmp_mask_reg (cond : Prop) `{Decision cond} (regs : Reg) (r : RegName) (pc_a : Addr)
+    (p : Perm) (b e a : Addr)
+    : coPset :=
+    if decide (reg_allows_IE_jmp regs r p b e a /\ cond)
+    then allow_jmp_mask pc_a a (a ^+1)%a
+    else (⊤ ∖ ↑logN.@pc_a).
+
+  (* The necessary resources to close the region again,
+     except for the points to predicate, which we will store separately *)
+  Definition region_open_resources2
+    (pc_a : Addr) (a a' : Addr)
+    (w1 : Word) (w2 : Word)
+    (P1 P2 : D)
+    : iProp Σ :=
+    ▷ P1 w1 ∗ ▷ P2 w2
+       ∗ persistent_cond P1 ∗ persistent_cond P2
+       ∗ ((▷ ∃ w1 w2, a ↦ₐ w1 ∗ P1 w1 ∗ a' ↦ₐ w2 ∗ P2 w2)
+          ={allow_jmp_mask pc_a a a', ⊤ ∖ ↑logN.@pc_a}=∗ emp)%I.
+
+  Definition region_open_resources
+    (pc_a : Addr) (a a' : Addr) (w : Word)
+    (P : D)
+    : iProp Σ :=
+    (▷ P w
+       ∗ persistent_cond P
+       ∗ ((▷ ∃ w, a ↦ₐ w ∗ P w)
+        ={allow_jmp_mask pc_a a a', ⊤ ∖ ↑logN.@pc_a}=∗ emp))%I.
+
+  Definition allow_jmp_res_mem
+    (pc_a : Addr) (a : Addr)
+    (P1 P2 : D): iProp Σ :=
+    (|={⊤ ∖ ↑logN.@pc_a, allow_jmp_mask pc_a a (a ^+1)%a}=>
+       (if decide (pc_a = a)
+        then ∃ w2, (a^+1)%a ↦ₐ w2 ∗ region_open_resources pc_a (a ^+1)%a a w2 P2
+        else
+          if decide (pc_a = (a^+1)%a)
+          then ∃ w1, a ↦ₐ w1 ∗ region_open_resources pc_a a (a ^+1)%a w1 P1
+          else ∃ w1 w2, a ↦ₐ w1 ∗ (a^+1)%a ↦ₐ w2 ∗ region_open_resources2 pc_a a (a ^+1)%a w1 w2 P1 P2)
+    )%I.
+
+  (* Description of what the resources are supposed to look like after opening the
+     region if we need to, but before closing the region up again*)
+  Definition allow_jmp_res (cond : Prop) `{Decision cond} (regs : Reg) (r : RegName)
+    (pc_a : Addr) (p : Perm) (b e a : Addr)
+    (P1 P2 : D): iProp Σ :=
+    (if decide (reg_allows_IE_jmp regs r p b e a /\ cond)
+       then
+         (∀ w1 w2 regs', ▷ □ (P1 w1 ∗ (P2 w2 ∨ ⌜ is_int w2 ⌝) -∗ (interp_expr_gen interp regs' w1 w2)))
+           ∗ allow_jmp_res_mem pc_a a P1 P2
+       else True)%I.
+
+  Lemma create_jmp_res (cond : Prop) `{Decision cond}:
+    ∀ (regs : leibnizO Reg) (r : RegName)
+      (pc_p : Perm) (pc_b pc_e pc_a : Addr)
+      (p : Perm) (b e a : Addr),
+      pc_p <> IE ->
+      (∀ (r' : RegName) (w : Word), ⌜r' ≠ PC⌝ → ⌜regs !! r' = Some w⌝ → (fixpoint interp1) w)
+        -∗ ∃ (P1 P2 : D),
+             @allow_jmp_res cond _ (<[PC:=WCap pc_p pc_b pc_e pc_a]> regs) r pc_a p b e a P1 P2.
+  Proof.
+    intros regs r pc_p pc_b pc_e pc_a p b e a Hpc_p.
+    iIntros "#Hreg".
+    rewrite /allow_jmp_res.
+    case_decide as Hallows; cycle 1.
+    - by iExists (λne _, True%I), (λne _, True%I).
+    - rewrite /allow_jmp_mask.
+      destruct Hallows as [(Hreg & -> & Hwb & Hwb') Hcond].
+      assert (a <> (a^+1)%a) by (apply Is_true_true_1, andb_prop in Hwb as [_ Hge]; solve_addr).
+      assert ( withinBounds b e a /\ withinBounds b e (a^+1)%a) as Hwbs by auto.
+
+      assert (r ≠ PC) as Hneq by (destruct (decide (r = PC)) ; simplify_map_eq; auto).
+      rewrite lookup_insert_ne //= in Hreg.
+
+      iDestruct ("Hreg" $! r _ Hneq Hreg) as "Hvsrc".
+      rewrite fixpoint_interp1_eq /=.
+      iDestruct ("Hvsrc" $! Hwbs) as (P1 P2) "(Hpers_P1 & Hpers_P2 & Hinv_a & Hinv_a' & Hexec)".
+      iExists P1, P2.
+      iFrame "#".
+      iClear "Hexec".
+      rewrite /allow_jmp_res_mem.
+
+      case_decide as Ha; simplify_eq.
+      { (* pc_a = a *)
+        iMod (inv_acc (⊤ ∖ ↑logN.@a) with "Hinv_a'") as "[Hrefinv_a' Hcls_a']";[solve_ndisj|].
+        iDestruct "Hrefinv_a'" as (w2) "[>Ha' HPa']".
+        iExists w2.
+        iFrame "∗ #".
+        rewrite /allow_jmp_mask decide_True //= decide_False //= decide_True //=.
+      }
+
+      case_decide as Ha'; simplify_eq.
+      { (* pc_a = a+1 *)
+        iMod (inv_acc (⊤ ∖ ↑logN.@(a ^+ 1)%a) with "Hinv_a") as "[Hrefinv_a Hcls_a]";[solve_ndisj|].
+        iDestruct "Hrefinv_a" as (w2) "[>Ha HPa]".
+        iExists w2.
+        iFrame "∗ #".
+        rewrite /allow_jmp_mask decide_False //= decide_True //=.
+      }
+
+      (* pc_a ≠ a ∧ pc_a ≠ a+1 *)
+      iMod (inv_acc (⊤ ∖ ↑logN.@pc_a) with "Hinv_a") as "[Hrefinv_a Hcls_a]";[solve_ndisj|].
+      iMod (inv_acc (⊤ ∖ ↑logN.@pc_a ∖ ↑logN.@a) with "Hinv_a'") as "[Hrefinv_a' Hcls_a']";[solve_ndisj|].
+      iDestruct "Hrefinv_a" as (w1) "[>Ha HPa]".
+      iDestruct "Hrefinv_a'" as (w2) "[>Ha' HPa']".
+      iExists w1, w2.
+
+      rewrite /region_open_resources2 /allow_jmp_mask decide_False //= decide_False //=.
+      iFrame "∗ #".
+      iModIntro.
+      iIntros "Ha".
+      iDestruct "Ha" as (w1' w2') "(Hw1' & HP1' & Hw2' & HP2')".
+      iMod ("Hcls_a'" with "[Hw2' HP2']") as "_"; first (iExists _ ; iFrame).
+      iMod ("Hcls_a" with "[Hw1' HP1']") as "_"; first (iExists _ ; iFrame).
+      done.
+  Qed.
+
+  Definition allow_jmp_mem_res
+    (mem : Mem) (pc_a : Addr) (pc_w : Word) (a : Addr) (P1 P2 : D) :=
+    (if decide (pc_a = a)
+    then ∃ w2, ⌜mem = <[(a^+1)%a:=w2]> (<[pc_a:=pc_w]> ∅)⌝ ∗ region_open_resources pc_a (a^+1)%a a w2 P2
+    else
+      if decide (pc_a = (a^+1)%a)
+      then ∃ w1, ⌜mem = <[a:=w1]> (<[pc_a:=pc_w]> ∅)⌝ ∗ region_open_resources pc_a a (a^+1)%a w1 P1
+      else ∃ w1 w2,
+          ⌜mem = <[(a^+1)%a:=w2]> (<[a:=w1]> (<[pc_a:=pc_w]> ∅))⌝ ∗ region_open_resources2 pc_a a (a^+1)%a w1 w2 P1 P2)%I.
+
+  Definition allow_jmp_mem (cond : Prop) `{Decision cond}
+    (regs : Reg) (mem : Mem) (r : RegName)
+    (pc_a : Addr) (pc_w : Word) (p : Perm) (b e a : Addr) (P1 P2 : D) :=
+    (if decide (reg_allows_IE_jmp regs r p b e a /\ cond)
+       then allow_jmp_mem_res mem pc_a pc_w a P1 P2
+       else ⌜mem = <[pc_a:=pc_w]> ∅⌝)%I.
+
+  Lemma jmp_res_implies_mem_map (cond : Prop) `{Decision cond}:
+    ∀ (regs : leibnizO Reg) (r : RegName)
+      (pc_a : Addr) (pc_w : Word)
+      (p : Perm) (b e a: Addr)
+      (P1 P2:D),
+      read_reg_inr regs r p b e a
+      -> @allow_jmp_res cond _ regs r pc_a p b e a P1 P2
+      -∗ pc_a ↦ₐ pc_w
+      ={⊤ ∖ ↑logN.@pc_a, @allow_jmp_mask_reg cond _ regs r pc_a p b e a }=∗
+      ∃ mem : Mem,
+          @allow_jmp_mem cond _ regs mem r pc_a pc_w p b e a P1 P2
+            ∗ ▷ ([∗ map] a0↦w ∈ mem, a0 ↦ₐ w).
+  Proof.
+    intros regs r pc_a pc_w p b e a P1 P2 Hrinr.
+    iIntros "HJmpRes Hpc_a".
+    rewrite /allow_jmp_res /allow_jmp_mask /allow_jmp_mask_reg.
+
+    case_decide as Hdec ; cycle 1.
+    { rewrite /read_reg_inr in Hrinr.
+      iExists _.
+      iSplitL "HJmpRes".
+      + rewrite /allow_jmp_mem decide_False //=.
+      + iModIntro. iNext. by iApply memMap_resource_1.
+    }
+    destruct Hdec as [(Hreg & -> & Hwb & Hwb') Hcond].
+    assert (a <> (a^+1)%a) as Haeq by (apply Is_true_true_1, andb_prop in Hwb as [_ Hge]; solve_addr).
+    iDestruct "HJmpRes" as "[Hexec HJmpRes]".
+    iMod "HJmpRes" as "HJmpRes".
+    rewrite /allow_jmp_mask /allow_jmp_mem /allow_jmp_mem_res.
+
+    case_decide as Ha ; simplify_eq.
+    { (* pc_a = a *)
+      iDestruct "HJmpRes" as (w2) "[Ha' HJmpRest]".
+      iExists _.
+      iModIntro.
+      rewrite decide_True; [|by rewrite /reg_allows_IE_jmp].
+      iSplitL "HJmpRest"; eauto.
+      iNext ; rewrite memMap_resource_2ne; auto; iFrame.
+    }
+
+    case_decide as Ha' ; simplify_eq.
+    { (* pc_a = a+1 *)
+      iDestruct "HJmpRes" as (w1) "[Ha HJmpRest]".
+      iExists _.
+      iModIntro.
+      rewrite decide_True; [|by rewrite /reg_allows_IE_jmp].
+      iSplitL "HJmpRest"; eauto.
+      iNext ; rewrite memMap_resource_2ne; auto; iFrame.
+    }
+
+    (* pc_a ≠ a ∧ pc_a ≠ a+1 *)
+    iDestruct "HJmpRes" as (w1 w2) "(Ha & Ha' & HJmpRest)".
+    iExists _.
+    iModIntro.
+    rewrite decide_True; [|by rewrite /reg_allows_IE_jmp].
+    iSplitL "HJmpRest"; eauto.
+    iNext ; rewrite memMap_resource_3ne; auto; iFrame.
+  Qed.
+
+  (* Close the invariants, in case of fail*)
+  Lemma mem_map_recover_res
+    (mem : Mem) (pc_a a : Addr) (pc_w : Word) (P1 P2 : D):
+    (a ^+ 1)%a ≠ a ->
+    allow_jmp_mem_res mem pc_a pc_w a P1 P2
+    -∗ ([∗ map] a'↦w' ∈ mem, a' ↦ₐ w')
+    ={allow_jmp_mask pc_a a (a ^+1)%a, ⊤ ∖ ↑logN.@pc_a}=∗ pc_a ↦ₐ pc_w.
+  Proof.
+    iIntros (Hneq) "HJmpMem Hmem".
+
+    rewrite /allow_jmp_mem_res /allow_jmp_mask.
+    case_decide as Ha; simplify_eq.
+    { (* pc_a = a *)
+      iDestruct "HJmpMem" as (w2) "(->&Hres)". rewrite /region_open_resources.
+      rewrite memMap_resource_2ne; auto.
+      iDestruct "Hmem" as "(Ha0' & Ha0)".
+      iDestruct "Hres" as "(HP2 & _ & Hcls')".
+      rewrite /allow_jmp_mask.
+      rewrite decide_False //= decide_True //=.
+      iMod ("Hcls'" with "[HP2 Ha0']") as "_" ; [iNext ; iExists w2; iFrame|auto].
+    }
+
+    case_decide as Ha'; simplify_eq.
+    { (* pc_a = a+1 *)
+      iDestruct "HJmpMem" as (w1) "(->&Hres)". rewrite /region_open_resources.
+      rewrite memMap_resource_2ne; auto.
+      iDestruct "Hmem" as "(Ha0 & Ha0')".
+      iDestruct "Hres" as "(HP1 & _ & Hcls')".
+      rewrite /allow_jmp_mask.
+      rewrite decide_False //= decide_True //=.
+      iMod ("Hcls'" with "[HP1 Ha0]") as "_" ; [iNext ; iExists w1; iFrame|auto].
+    }
+
+    (* a ≠ a0 ∧ a ≠ a0+1 *)
+    iDestruct "HJmpMem" as (w1 w2) "(->&Hres)". rewrite /region_open_resources2.
+    rewrite memMap_resource_3ne; auto.
+    iDestruct "Hmem" as "(Ha0' & Ha0 & Ha)".
+    iDestruct "Hres" as "(HP1 & HP2 & _& _ & Hcls')".
+    rewrite /allow_jmp_mask.
+    rewrite decide_False //= decide_False //=.
+    iMod ("Hcls'" with "[HP1 HP2 Ha0 Ha0']") as "_"; [iNext ; iExists w1,w2; iFrame|auto].
+  Qed.
+
+  (* Close the invariants, in case of jump to IE *)
+  Lemma mem_map_recover_res_ie
+    (mem : Mem) (pc_a a : Addr) (pc_w wpc widc : Word) (P P1 P2 : D):
+    (a ^+ 1)%a ≠ a ->
+    mem !! a = Some wpc ->
+    mem !! (a ^+ 1)%a = Some widc ->
+
+    allow_jmp_mem_res mem pc_a pc_w a P1 P2
+    -∗ ([∗ map] a'↦w' ∈ mem, a' ↦ₐ w')
+    ={allow_jmp_mask pc_a a (a ^+1)%a, ⊤ ∖ ↑logN.@pc_a}=∗
+      if (decide (pc_a = a))
+      then pc_a ↦ₐ pc_w ∗ ⌜pc_w = wpc ⌝
+      else
+        if (decide (pc_a = (a^+1)%a))
+        then pc_a ↦ₐ widc ∗ ⌜pc_w = widc⌝ ∗ ▷ P1 wpc ∗ persistent_cond P1
+        else pc_a ↦ₐ pc_w ∗ ▷ P1 wpc ∗ ▷ P2 widc ∗ persistent_cond P1 ∗ persistent_cond P2.
+  Proof.
+    iIntros (Hneq Hmem_a Hmem_a') "HJmpMem Hmem".
+    rewrite /allow_jmp_mem_res /allow_jmp_mask.
+
+    case_decide as Ha; simplify_eq.
+    { (* a = a0 *)
+      iDestruct "HJmpMem" as (w2) "(->& HP2& %Hpers2& Hcls')".
+      rewrite /allow_jmp_mask.
+      rewrite decide_False //= decide_True //=.
+      rewrite memMap_resource_2ne; auto.
+      simplify_map_eq.
+      iDestruct "Hmem" as  "[Ha0' Ha0]".
+      iMod ("Hcls'" with "[HP2 Ha0']") as "_" ; [iNext;iExists widc;iFrame "∗ #"|auto].
+    }
+
+    case_decide as Ha'; simplify_eq.
+    { (* a = a0+1 *)
+      iDestruct "HJmpMem" as (w1) "(->& HP1& %Hpers1& Hcls')".
+      iDestruct "HP1" as "#HP1".
+      rewrite /allow_jmp_mask.
+      rewrite decide_False //= decide_True //=.
+      rewrite memMap_resource_2ne; auto.
+      simplify_map_eq.
+      iDestruct "Hmem" as "[Ha0' Ha0]".
+      iMod ("Hcls'" with "[HP1 Ha0']") as "_" ; [iNext;iExists wpc;iFrame "∗ #"|auto].
+    }
+
+    (* a ≠ a0 ∧ a ≠ a0+1 *)
+    iDestruct "HJmpMem" as (w1 w2) "(->& HP1& HP2& %Hpers1& %Hpers2& Hcls')".
+    rewrite /region_open_resources2.
+    iDestruct "HP1" as "#HP1"; iDestruct "HP2" as "#HP2".
+    rewrite /allow_jmp_mask; case_decide ; simplify_eq; case_decide ; simplify_eq.
+    rewrite memMap_resource_3ne; auto.
+    simplify_map_eq.
+    iDestruct "Hmem" as  "(Ha0' & Ha0 & Ha)".
+    iMod ("Hcls'" with "[HP1 HP2 Ha0' Ha0]") as "_"; [iNext;iExists wpc,widc;iFrame "∗ #"|auto].
+  Qed.
+
+  (* Derice pure conds =allow_jmp_mmap_or_true= from =cond_jmp= *)
+  Lemma mem_map_implies_pure_conds:
+    ∀ (regs : leibnizO Reg) (mem : Mem) (r : RegName)
+      (pc_a : Addr) (pc_w : Word)
+      (p : Perm) (b e a : Addr) (P1 P2 : D),
+      read_reg_inr regs r p b e a
+      -> allow_jmp_mem cond_jmp regs mem r pc_a pc_w p b e a P1 P2
+      -∗ ⌜mem !! pc_a = Some pc_w⌝ ∗ ⌜allow_jmp_mmap_or_true cond_jmp r regs mem⌝.
+  Proof.
+    iIntros (regs mem r pc_a pc_w p b e a P1 P2 Hrinr) "HJmpMem".
+    rewrite /allow_jmp_mem.
+    case_decide as Hdec ; cycle 1.
+    { iDestruct "HJmpMem" as "->".
+      iSplitR. by rewrite lookup_insert.
+      iExists p,b,e,a.
+      iSplitR; auto.
+      rewrite decide_False //=.
+    }
+    destruct Hdec as [Hdec _].
+
+    rewrite /allow_jmp_mem_res.
+    assert (a <> (a^+1)%a)
+    by (inversion Hdec as (_ & _ & Hwb%Is_true_true_1%withinBounds_true_iff & _); solve_addr).
+
+    case_decide as Ha; simplify_eq.
+    { (* pc_a = a *)
+      iDestruct "HJmpMem" as (w2) "[%Hmem _]" ; subst.
+      iSplitL.
+      by iPureIntro; simplify_map_eq.
+      iExists p,b,e,a.
+      iSplitR; auto.
+      case_decide; auto.
+      inversion Hdec.
+      iExists pc_w, w2.
+      by iPureIntro ; split ; simplify_map_eq.
+    }
+
+    case_decide as Ha'; simplify_eq.
+    { (* pc_a = a+1 *)
+      iDestruct "HJmpMem" as (w1) "[%Hmem _]" ; subst.
+      iSplitL.
+      by iPureIntro; simplify_map_eq.
+      iExists p,b,e,a.
+      iSplitR; auto.
+      case_decide; auto.
+      inversion Hdec.
+      iExists w1, pc_w.
+      by iPureIntro ; split ; simplify_map_eq.
+    }
+
+    (* pc_a ≠ a ∧ pc_a ≠ a+1 *)
+    iDestruct "HJmpMem" as (w1 w2) "[%Hmem _]" ; subst.
+    iSplitL.
+    by iPureIntro; simplify_map_eq.
+    iExists p,b,e,a.
+    iSplitR; auto.
+    case_decide; auto.
+    inversion Hdec.
+    iExists w1, w2.
+    by iPureIntro ; split ; simplify_map_eq.
+  Qed.
+
+  Lemma jmpiepair_case (regs : leibnizO Reg) (p : Perm)
+        (b e a : Addr) (widc w : Word) (src : RegName) (P : D):
+    ftlr_instr regs p b e a widc w (JmpIEpair src) P.
+  Proof.
+    intros Hp Hsome i Hbae Hi.
+    iIntros
+      "#IH #Hinv_pc #Hinv_idc #Hinva #Hreg #[Hread _] Hown Ha HP Hcls HPC HIDC Hmap".
+    iInsertList "Hmap" [idc;PC].
+
+    (* To read out PC's name later, and needed when calling wp_load *)
+    assert(∀ x : RegName, is_Some (<[PC:=WCap p b e a]> (<[idc:=widc]> regs) !! x)) as Hsome'.
+    {
+      intros. destruct (decide (x = PC)).
+      rewrite e0 lookup_insert; unfold is_Some. by eexists.
+      destruct (decide (x = idc)).
+      rewrite lookup_insert_ne; auto.
+      rewrite e0 lookup_insert; unfold is_Some. by eexists.
+      by rewrite! lookup_insert_ne.
+    }
+
+    (* Initializing the names for the values of Hsrc now, to instantiate the existentials in step 1 *)
+    assert (∃ p0 b0 e0 a0, read_reg_inr (<[PC:=WCap p b e a]> (<[idc:=widc]> regs)) src p0 b0 e0 a0)
+      as [p0 [b0 [e0 [a0 HVsrc] ] ] ].
+    {
+      specialize Hsome' with src as Hsrc.
+      destruct Hsrc as [wsrc Hsomesrc].
+      unfold read_reg_inr. rewrite Hsomesrc.
+      destruct wsrc as [|[ p0 b0 e0 a0|] | ]; try done.
+      by repeat eexists.
+    }
+
+    iAssert (∀ (r' : RegName) (w : Word),
+                ⌜r' ≠ PC⌝ → ⌜<[idc:=widc]> regs  !! r' = Some w⌝ → fixpoint interp1 w)%I
+      as "Hreg'".
+    { iIntros.
+      destruct (decide (r' = idc)); simplify_map_eq; auto.
+      iApply "Hreg";eauto.
+    }
+
+    (* Step 1: open the region, if necessary, and store all the resources
+       obtained from the region in allow_IE_res *)
+    iDestruct ((create_jmp_res cond_jmp _ _ p)  with "Hreg'") as (P1 P2) "HJmpRes"; eauto.
+    { destruct Hp ; destruct p ; eauto. }
+
+    (* Step2: derive the concrete map of memory we need, and any spatial
+       predicates holding over it *)
+    iMod ((jmp_res_implies_mem_map cond_jmp) with "HJmpRes Ha") as (mem) "[HJmpMem HJmpRest]"; first eauto.
+
+    (* Step 3:  derive the non-spatial conditions over the memory map*)
+    iDestruct (mem_map_implies_pure_conds with "HJmpMem") as
+      %(HReadPC & HAJmpMem); auto.
+
+    (* Step 3.5:  derive the non-spatial conditions over the registers *)
+    assert (allow_jmp_rmap_or_true cond_jmp src
+               (<[PC:=WCap p b e a]> (<[idc:=widc]> regs))) as HAJmpReg.
+    { rewrite /allow_jmp_rmap_or_true.
+      exists p0, b0, e0, a0.
+      split; auto.
+      case_decide as Heq; auto.
+      by exists widc; simplify_map_eq.
+    }
+
+    iApply (wp_jmpIEpair with "[Hmap HJmpRest]");eauto.
+    { by simplify_map_eq. }
+    { rewrite /subseteq /map_subseteq /set_subseteq_instance. intros rr _.
+      apply elem_of_dom. repeat (rewrite lookup_insert_is_Some'; right); eauto. }
+    { iSplitR "Hmap"; auto. }
+
+    iNext. iIntros (regs' retv). iDestruct 1 as (HSpec) "[Hmem Hmap]".
+    (* Infer that if P holds at w, then w must be valid (read condition) *)
+    iDestruct ("Hread" with "HP") as "#Hw".
+
+    destruct HSpec as [* Hregs Hwb Hwb' Ha Ha' HincrPC | Hfail].
+    - (* success jmp IE *)
+      rewrite insert_insert insert_commute //= insert_insert in HincrPC; subst regs'.
+
+      assert (p0 = IE /\ b0 = b1 /\ e0 = e1 /\ a0 = a1) as (-> & <- & <- & <-)
+          by (by rewrite /read_reg_inr in HVsrc; rewrite Hregs in HVsrc; simplify_eq).
+      assert ((a0 ^+ 1)%a ≠ a0) as Haeq by (apply Is_true_true_1, withinBounds_true_iff in Hwb ; solve_addr).
+      assert (withinBounds b0 e0 a0 ∧ withinBounds b0 e0 (a0 ^+ 1)%a) as Hbounds by auto.
+      assert (PC <> src) as Hsrc
+          by (destruct (decide (PC = src)); auto; simplify_map_eq; by
+                destruct Hp).
+      assert (reg_allows_IE_jmp
+                (<[PC:=WCap p b e a]> (<[idc:=widc]> regs))
+                src IE b0 e0 a0) as HallowJmp
+          by (by rewrite /reg_allows_IE_jmp; auto).
+
+      rewrite /allow_jmp_res /allow_jmp_mask_reg.
+      rewrite !decide_True //=.
+      iDestruct "HJmpRes" as "(Hexec&HJmpRes)".
+      rewrite /allow_jmp_mem.
+      rewrite !decide_True //=.
+
+      (* Step 4: return all the resources we had *)
+      iMod ((mem_map_recover_res_ie _ _ _ w wpc widc0 P P1 P2) with "HJmpMem Hmem") as "Ha"
+      ; auto; iModIntro.
+
+      case_decide as Ha0; simplify_eq.
+      { (* a = a0 *)
+
+        iDestruct "Ha" as "[Ha0 ->]".
+
+        iMod ("Hcls" with "[HP Ha0]") as "_"; [iNext;iExists wpc;iFrame|iModIntro].
+        iApply wp_pure_step_later; auto.
+        iNext ; iIntros "_".
+        destruct wpc; cbn in Hi; try done.
+        iExtract "Hmap" PC as "HPC".
+        iApply interp_expr_invalid_pc; try iFrame ; eauto.
+        intro Hcontra; inversion Hcontra ; simplify_eq.
+        iPureIntro; apply regmap_full_dom in Hsome; rewrite -Hsome; set_solver.
+      }
+
+      case_decide as Ha0'; simplify_eq.
+      { (* a = a0+1 *)
+
+        iDestruct "Ha" as "(Ha0 & -> & HP1 & %Hpers1)".
+        iDestruct "HP1" as "#HP1".
+
+        iMod ("Hcls" with "[HP Ha0]") as "_"; [iNext;iExists widc0;iFrame|iModIntro].
+        iApply wp_pure_step_later; auto.
+        iNext ; iIntros "_".
+        iApply ("Hexec" $! _ widc0) ; iFrame "∗ #".
+        iRight; destruct widc0; cbn in Hi; try done.
+        rewrite insert_commute //=.
+        repeat (iSplit ; try done).
+      }
+
+      (* a ≠ a0 ∧ a ≠ a0+1 *)
+      iDestruct "Ha" as "(Ha & HP1 & HP2 & %Hpers1 & %Hpers2)".
+      iDestruct "HP1" as "#HP1"; iDestruct "HP2" as "#HP2".
+      iMod ("Hcls" with "[HP Ha]") as "_"; [iNext;iExists w;iFrame|iModIntro].
+      iApply wp_pure_step_later; auto.
+      iNext; iIntros "_".
+      iApply "Hexec" ; iFrame "∗ #".
+      rewrite insert_commute //=.
+      repeat (iSplit ; try done).
+
+    - (* fail *)
+      rewrite /allow_jmp_mask_reg /allow_jmp_mem /allow_jmp_res.
+      destruct (decide ((reg_allows_IE_jmp
+                          (<[PC:=WCap p b e a]> (<[idc:=widc]> regs))
+                          src p0 b0 e0 a0) /\ cond_jmp)) as [HallowJmp|_]
+      ; cycle 1.
+      {
+        iModIntro.
+        iDestruct "HJmpMem" as "->". rewrite -memMap_resource_1.
+        iMod ("Hcls" with "[Hmem HP]") as "_";[iExists w;iFrame|iModIntro].
+        iApply wp_pure_step_later; auto.
+        iNext; iIntros "_".
+        iApply wp_value; auto; iIntros; discriminate.
+      }
+
+      assert ((a0 ^+ 1)%a ≠ a0) as Ha0eq
+      by (destruct HallowJmp as
+           [(_ & _ & Hwb%Is_true_true_1%withinBounds_true_iff & _) _]; solve_addr).
+
+      (* Step 4: return all the resources we had *)
+      iMod (mem_map_recover_res with "HJmpMem Hmem") as "Ha"; auto.
+
+      iModIntro.
+      iMod ("Hcls" with "[Ha HP]") as "_";[iExists w;iFrame|iModIntro].
+      iApply wp_pure_step_later; auto.
+      iNext; iIntros "_".
+      iApply wp_value; auto; iIntros; discriminate.
+    Qed.
+
+End fundamental.
