theories/ftlr/Jnz.v
@@ -3,7 +3,7 @@ From iris.program_logic Require Import weakestpre adequacy lifting.
 From stdpp Require Import base.
 From cap_machine Require Export logrel register_tactics.
 From cap_machine.rules Require Import rules_Jnz.
-From cap_machine.ftlr Require Import ftlr_base Jmp.
+From cap_machine.ftlr Require Import ftlr_base interp_weakening.
 
 Section fundamental.
   Context {Σ:gFunctors} {memg:memG Σ} {regg:regG Σ} {sealsg: sealStoreG Σ}
@@ -15,69 +15,6 @@ Section fundamental.
   Implicit Types w : (leibnizO Word).
   Implicit Types interp : (D).
 
-  (* Derice pure conds =allow_jnz_mmap_or_true= from =cond_jnz= *)
-  Lemma mem_map_implies_pure_conds:
-    ∀ (regs : Reg) (mem : Mem) (dst src : RegName)
-      (pc_a : Addr) (pc_w : Word)
-      (p : Perm) (b e a : Addr) (wsrc : Word)
-      (P1 P2 : D),
-      read_reg_inr regs dst p b e a
-      -> regs !! src = Some wsrc
-      -> allow_jmp_mem (cond_jnz regs src wsrc) regs mem dst pc_a pc_w p b e a P1 P2
-        -∗ ⌜mem !! pc_a = Some pc_w⌝
-          ∗ ⌜allow_jmp_mmap_or_true (cond_jnz regs src wsrc) dst regs mem⌝.
-  Proof.
-    iIntros (regs mem dst src pc_a pc_w p b e a wsrc P1 P2 Hrinr Hsrc) "HJmpMem".
-    rewrite /allow_jmp_mem.
-    case_decide as Hdec ; cycle 1.
-    { iDestruct "HJmpMem" as "->".
-      iSplitR. by rewrite lookup_insert.
-      iPureIntro.
-      exists p,b,e,a.
-      split; auto.
-      rewrite decide_False //=.
-    }
-    destruct Hdec as (Hdec & Hjnz).
-
-    rewrite /allow_jmp_mem_res.
-    assert (a <> (a^+1)%a)
-    by (inversion Hdec as (_ & _ & Hwb%Is_true_true_1%withinBounds_true_iff & _); solve_addr).
-
-    case_decide as Ha; simplify_eq.
-    { (* pc_a = a *)
-      iDestruct "HJmpMem" as (w2) "[%Hmem _]" ; subst.
-      iSplitL; iPureIntro.
-      by simplify_map_eq.
-      exists p,b,e,a.
-      split;auto.
-      rewrite decide_True //=.
-      exists pc_w, w2.
-      by split ; simplify_map_eq.
-    }
-
-    case_decide as Ha'; simplify_eq.
-    { (* pc_a = a+1 *)
-      iDestruct "HJmpMem" as (w1) "[%Hmem _]" ; subst.
-      iSplitL; iPureIntro.
-      by simplify_map_eq.
-      exists p,b,e,a.
-      split;auto.
-      rewrite decide_True //=.
-      exists w1, pc_w.
-      by split ; simplify_map_eq.
-    }
-
-    (* pc_a ≠ a ∧ pc_a ≠ a+1 *)
-    iDestruct "HJmpMem" as (w1 w2) "[%Hmem _]" ; subst.
-    iSplitL; iPureIntro.
-    by simplify_map_eq.
-    exists p,b,e,a.
-    split;auto.
-    rewrite decide_True //=.
-    exists w1, w2.
-    by split ; simplify_map_eq.
-  Qed.
-
   Lemma jnz_case (regs : Reg) (p : Perm)
         (b e a : Addr) (widc w : Word) (dst src : RegName) (P : D):
     ftlr_instr regs p b e a widc w (Jnz dst src) P.
@@ -87,309 +24,99 @@ Section fundamental.
       "#IH #Hinv_pc #Hinv_idc #Hinva #Hreg #[Hread _] Hown Ha HP Hcls HPC HIDC Hmap".
     iInsertList "Hmap" [idc;PC].
 
-    (* To read out PC's name later, and needed when calling wp_load *)
-    assert(∀ x : RegName, is_Some (<[PC:=WCap p b e a]> (<[idc:=widc]> regs) !! x)) as Hsome'.
-    {
-      intros. destruct (decide (x = PC)).
-      rewrite e0 lookup_insert; unfold is_Some. by eexists.
-      destruct (decide (x = idc)).
-      rewrite lookup_insert_ne; auto.
-      rewrite e0 lookup_insert; unfold is_Some. by eexists.
-      by rewrite! lookup_insert_ne.
-    }
-
-    (* Initializing the names for the values of Hsrc now, to instantiate the existentials in step 1 *)
-    assert (∃ p0 b0 e0 a0, read_reg_inr (<[PC:=WCap p b e a]> (<[idc:=widc]> regs)) dst p0 b0 e0 a0)
-      as [p0 [b0 [e0 [a0 HVdst] ] ] ].
-    {
-      specialize Hsome' with dst as Hdst.
-      destruct Hdst as [wdst Hsomedst].
-      unfold read_reg_inr. rewrite Hsomedst.
-      destruct wdst as [|[ p0 b0 e0 a0|] | ]; try done.
-      by repeat eexists.
-    }
-
-    assert (exists wsrc, (<[PC:=WCap p b e a]> (<[idc:=widc]> regs)) !! src = Some wsrc) as [wsrc HVsrc].
-    {
-      specialize Hsome' with src as Hsrc.
-      destruct Hsrc as [wsrc Hsomesrc].
-      by eexists.
-    }
-
-    iAssert (
-        ∀ (r' : RegName) (w : Word),
-          ⌜r' ≠ PC⌝ → ⌜<[idc:=widc]> regs  !! r' = Some w⌝ → fixpoint interp1 w
-      )%I as "Hreg'".
-    { iIntros.
-      destruct (decide (r' = idc)); simplify_map_eq; auto.
-      iApply "Hreg";eauto.
-    }
-
-    set (Hcond_jnz := cond_jnz (<[PC:=WCap p b e a]> (<[idc:=widc]> regs)) src wsrc).
-
-    (* Step 1: open the region, if necessary, and store all the resources
-       obtained from the region in allow_IE_res *)
-    iDestruct ((create_jmp_res Hcond_jnz _ _ p)  with "Hreg'") as (P1 P2) "HJmpRes"; eauto.
-    { destruct Hp ; destruct p ; auto. }
-
-    (* Step2: derive the concrete map of memory we need, and any spatial
-       predicates holding over it *)
-    iMod ((jmp_res_implies_mem_map Hcond_jnz)
-           with "HJmpRes Ha") as (mem) "[HJmpMem HJmpRest]"; eauto.
-
-    (* Step 3:  derive the non-spatial conditions over the memory map*)
-    iDestruct ((mem_map_implies_pure_conds _ mem dst src a w p0 b0 e0 a0 wsrc P1 P2)
-                with "HJmpMem") as %(HReadPC & HAJmpMem); eauto.
-
-    (* Step 3.5:  derive the non-spatial conditions over the registers *)
-    assert (allow_jmp_rmap_or_true Hcond_jnz dst (<[PC:=WCap p b e a]> (<[idc:=widc]> regs)))
-      as HAJmpReg.
-    { rewrite /allow_jmp_rmap_or_true.
-      exists p0, b0, e0, a0.
-      split; auto.
-      (* TODO any way to avoid manual match ? *)
-      match goal with
-      | H: _ |- (if (decide ?cond) then _ else _) =>
-          destruct (decide cond)
-      end; auto.
-      by eexists _; simplify_map_eq.
-    }
-
-    assert (
-        regs_of (Jnz dst src) ⊆ dom (<[PC:=WCap p b e a]> (<[idc:=widc]> regs))
-      ).
+    iApply (wp_Jnz with "[$Ha $Hmap]"); eauto.
+    { simplify_map_eq; auto. }
     { rewrite /subseteq /map_subseteq /set_subseteq_instance. intros rr _.
-      apply elem_of_dom. repeat (rewrite lookup_insert_is_Some'; right); eauto. }
-    iApply (wp_Jnz _ _ _ _ _ _ _ _ (<[PC:=WCap p b e a]> (<[idc:=widc]> regs))
-             with "[Hmap HJmpRest]");eauto.
-    { by simplify_map_eq. }
-    { iSplitR "Hmap"; auto. }
-    iNext. iIntros (regs' retv). iDestruct 1 as (HSpec) "[Hmem Hmap]".
-    (* Infer that if P holds at w, then w must be valid (read condition) *)
-    iDestruct ("Hread" with "HP") as "#Hw".
-    rewrite /allow_jmp_res /allow_jmp_mem /allow_jmp_mask_reg /allow_jmp_mask.
+      apply elem_of_dom. repeat (apply lookup_insert_is_Some'; right ; eauto). }
+
+    iIntros "!>" (regs' retv). iDestruct 1 as (HSpec) "[Hmem Hmap]".
 
     destruct HSpec as
-      [ Hfail
-      | * Hsrc Hdst Hcond Hwb Hwb' Ha Ha' HincrPC (* Success IE true *)
-      | * Hsrc Hdst Hcond HnIE HincrPC (* Success true *)
+      [ * Hsrc Hcond HincrPC (* Fail *)
       | * Hsrc Hcond HincrPC (* Success false *)
+      | * Hsrc Hdst Hcond (* Success true *)
       ].
-    - (* Fail *)
-      match goal with
-      | H: _ |- context [(if (decide ?cond) then _ else _)] =>
-          destruct (decide cond) as [HallowJmp|HallowJmp] ; cycle 1
-      end; auto.
-      {
-        iModIntro.
-        iDestruct "HJmpMem" as "->". rewrite -memMap_resource_1.
-        iMod ("Hcls" with "[Hmem HP]") as "_";[iExists w;iFrame|iModIntro].
-        iApply wp_pure_step_later; auto.
-        iNext; iIntros "_".
-        iApply wp_value; auto; iIntros; discriminate.
-      }
-      destruct HallowJmp as (HallowJmp & _).
-      assert ((a0 ^+ 1)%a ≠ a0) as Ha0eq
-          by (destruct HallowJmp as (_ & _ & Hwb%Is_true_true_1%withinBounds_true_iff & _); solve_addr).
-      rewrite /allow_jmp_mem_res /allow_jmp_mask.
 
-      (* Step 4: return all the resources we had *)
-      iMod (mem_map_recover_res with "HJmpMem Hmem") as "Ha"; auto.
+    (* Hfail *)
+    {
+      iApply wp_pure_step_later;  auto.
+      iMod ("Hcls" with "[Hmem HP]");[iExists w;iFrame|iModIntro]. iNext.
+      iIntros "_".
+      iApply wp_value; auto. iIntros; discriminate.
+    }
 
+    (* Hsuccess false *)
+    { match goal with
+      | H: incrementPC _ = Some _ |- _ => apply incrementPC_Some_inv in H as (p''&b''&e''&a''& ? & HPC & Z & Hregs')
+      end. simplify_map_eq. rewrite insert_insert.
+      iApply wp_pure_step_later; auto.
+      iMod ("Hcls" with "[Hmem HP]");[iExists w;iFrame|iModIntro]. iNext.
+      iIntros "_".
+      iApply ("IH" $! regs _ _ _ x with "[%] [] [Hmap] [$Hown]"); eauto.
+      { rewrite insert_commute //=. }
       iModIntro.
-      iMod ("Hcls" with "[Ha HP]") as "_";[iExists w;iFrame|iModIntro].
-      iApply wp_pure_step_later; auto.
-      iNext; iIntros "_".
-      iApply wp_value; auto; iIntros; discriminate.
+      iApply (interp_weakening with "IH"); eauto.
+      by destruct Hp as [-> | ->].
+      by destruct Hp as [-> | ->].
+      solve_addr.
+      solve_addr.
+      by rewrite PermFlowsToReflexive.
+    }
 
-    - (* Success IE true*)
-      rewrite insert_insert insert_commute //= insert_insert in HincrPC; subst regs'.
-      match goal with
-      | H: _ |- context [(if (decide ?cond) then _ else _)] =>
-          destruct (decide cond) as [HallowJmp|HallowJmp]
-      end; auto.
-      2: { (* contradiction *)
-        rewrite /reg_allows_IE_jmp in HallowJmp.
-        rewrite /read_reg_inr in HVdst.
-        rewrite Hdst in HVdst; simplify_eq.
-        repeat (apply not_and_r in HallowJmp as [HallowJmp|HallowJmp] ; simplify_eq)
-        ; try congruence.
-        exfalso. apply HallowJmp.
-        by rewrite /Hcond_jnz /cond_jnz; intros _.
-      }
-      destruct HallowJmp as (HallowJmp & _).
-      assert (PC <> dst) as Hdst'
-          by (destruct (decide (PC = dst)); auto; simplify_map_eq; by destruct Hp).
-      assert (p0 = IE /\ b0 = b1 /\ e0 = e1 /\ a0 = a1) as (-> & <- & <- & <-)
-          by (by eapply reg_allows_IE_jmp_same)
-      ; simplify_map_eq.
-      assert ((a0 ^+ 1)%a ≠ a0) as Haeq by (apply Is_true_true_1, withinBounds_true_iff in Hwb ; solve_addr).
-      assert (withinBounds b0 e0 a0 ∧ withinBounds b0 e0 (a0 ^+ 1)%a) as Hbounds
-          by auto.
+    (* Hsuccess true *)
+    { simplify_map_eq. iApply wp_pure_step_later; auto.
+      rewrite !insert_insert.
 
-      iDestruct "HJmpRes" as "(Hexec&HJmpRes)".
+      iMod ("Hcls" with "[HP Hmem]");[iExists w;iFrame|iModIntro].
 
-      (* Step 4: return all the resources we had *)
-      iMod ((mem_map_recover_res_ie _ _ _ w wpc widc0 P P1 P2) with "HJmpMem Hmem") as "Ha"
-      ; auto; iModIntro.
-
-
-      destruct_decide (decide (a = a0)) as Ha0; simplify_eq.
-      { (* a = a0 *)
-
-        iDestruct "Ha" as "[Ha0 ->]".
-
-        iMod ("Hcls" with "[HP Ha0]") as "_"; [iNext;iExists wpc;iFrame|iModIntro].
-        iClear "HJmpRes".
-        iApply wp_pure_step_later; auto.
-        iNext ; iIntros "_".
-        destruct wpc; cbn in Hi; try done.
-        iExtract "Hmap" PC as "HPC".
-        iApply interp_expr_invalid_pc; try iFrame ; eauto.
-        intro Hcontra; inversion Hcontra.
-        iPureIntro; apply regmap_full_dom in Hsome; rewrite -Hsome; set_solver.
-      }
-
-      destruct_decide (decide (a = (a0 ^+ 1)%a)) as Ha0'; simplify_eq.
-      { (* a = a0+1 *)
-
-        iDestruct "Ha" as "(Ha0 & -> & HP1 & %Hpers1)".
-        iDestruct "HP1" as "#HP1".
-
-        iMod ("Hcls" with "[HP Ha0]") as "_"; [iNext;iExists widc0;iFrame|iModIntro].
-        iApply wp_pure_step_later; auto.
-        iNext ; iIntros "_".
-        iApply ("Hexec" $! _ widc0) ; iFrame "∗ #".
-        iRight; destruct widc0; cbn in Hi; try done.
-        rewrite insert_commute //=.
-        repeat (iSplit ; try done).
-      }
-
-      (* a ≠ a0 ∧ a ≠ a0+1 *)
-      iDestruct "Ha" as "(Ha & HP1 & HP2 & %Hpers1 & %Hpers2)".
-      iDestruct "HP1" as "#HP1"; iDestruct "HP2" as "#HP2".
-      iMod ("Hcls" with "[HP Ha]") as "_"; [iNext;iExists w;iFrame|iModIntro].
-      iApply wp_pure_step_later; auto.
-      iNext; iIntros "_".
-      iApply "Hexec" ; iFrame "∗ #".
-      rewrite insert_commute //=.
-      repeat (iSplit ; try done).
-
-    - (* Success true *)
-      rewrite insert_insert in HincrPC; subst regs'.
-      match goal with
-      | H: _ |- context[(if (decide ?cond) then _ else _)]=>
-          destruct_decide (decide cond) as HallowJmp
-      end; auto.
-      { (* contradiction *)
-        rewrite /reg_allows_IE_jmp in HallowJmp.
-        destruct HallowJmp as ((Hregs0 & -> & Hwb & Hwb') & _).
-        rewrite Hregs0 in Hdst.
-        simplify_map_eq.
-      }
-      iModIntro.
-      iDestruct "HJmpMem" as "->". rewrite -memMap_resource_1.
-      iMod ("Hcls" with "[Hmem HP]") as "_";[iExists w;iFrame|iModIntro].
-      iApply wp_pure_step_later; auto.
-
-      set (regs' := <[PC:=updatePcPerm w0]> (<[idc:=widc]> regs)).
       (* Needed because IH disallows non-capability values *)
       destruct w' as [ | [p' b' e' a' | ] | ]; cycle 1.
       {
         rewrite /updatePcPerm.
-        set (pc_p' := if decide (p' = E) then RX else p').
-
-        destruct (decide (p' = E)); simplify_map_eq.
-        (* Special case if p' is E *)
-        - (* p' = E *)
-          iAssert (interp (WCap E b' e' a')) as "Hinterp".
-          {
-          assert ( dst <> PC ).
-          { destruct (decide (dst = PC)) ; simplify_map_eq ; destruct Hp; auto. }
-          simplify_map_eq.
-          destruct (decide (dst = idc)) ; simplify_map_eq; auto.
-          iApply "Hreg"; auto.
+        iAssert (fixpoint interp1 (WCap p' b' e' a')) as "HECap".
+        { destruct (decide (dst = PC)) as [-> | Hne]. by simplify_map_eq.
+          rewrite lookup_insert_ne // in Hdst.
+          { destruct (decide (dst = idc)) as [-> | Hne']. by simplify_map_eq.
+            rewrite lookup_insert_ne // in Hdst.
+            iApply "Hreg"; eauto.
           }
-          rewrite (fixpoint_interp1_eq (WCap E _ _ _)) //=.
-          rewrite (insert_commute _ PC _ (WCap RX _ _ _)) //=.
-          iDestruct ("Hinterp" with "[$Hinv_idc] [$Hmap $Hown]") as "Hcont"; auto.
-        - (* p' ≠ E *)
-        iNext ; iIntros "_".
-        iApply ("IH" $! regs' pc_p' with "[%] [] [Hmap] [$Hown]"); subst regs'.
-        { intro; cbn; by repeat (rewrite lookup_insert_is_Some'; right). }
-        { iIntros (ri v Hri Hri' Hvs).
-          simplify_map_eq.
-          iApply "Hreg"; auto.
         }
-        { rewrite
-            insert_insert
-              (insert_commute _ idc) //=
-              insert_insert.
-          subst pc_p'; simplify_eq.
-          by destruct p'.
-        }
-        { iModIntro.
-          subst pc_p'.
-          iClear "HJmpRes IH Hread".
-          clear Hsome' HVdst HAJmpMem HAJmpReg.
 
-          destruct (decide (dst = PC)); simplify_map_eq; auto.
-          destruct (decide (dst = idc)); simplify_map_eq; auto.
-          iApply "Hreg" ; auto.
-        }
-        { iFrame "Hinv_idc". }
+        (* Special case for E-values*)
+        destruct (decide (p' = E)) as [-> | HneE].
+        - iEval (rewrite fixpoint_interp1_eq; simpl) in "HECap".
+          rewrite insert_commute //=.
+
+          iDestruct ("HECap" with "[$Hinv_idc] [$Hmap $Hown]") as "Hcont"; auto.
+        - iAssert ([∗ map] k↦y ∈ <[PC:= WCap p' b' e' a']> (<[idc:=widc]> regs), k ↦ᵣ y)%I  with "[Hmap]" as "Hmap".
+          { destruct p'; auto. congruence. }
+          iNext; iIntros "_".
+
+          iApply ("IH" $! (<[PC:=WCap p' b' e' a']> (<[idc:=widc]> regs)) with "[%] [] [Hmap] [$Hown]").
+          { cbn. intros. by repeat (rewrite lookup_insert_is_Some'; right). }
+          { iIntros (ri v Hri Hri' Hvs).
+            rewrite lookup_insert_ne in Hvs; auto.
+            iApply "Hreg"; eauto. by simplify_map_eq. }
+          { rewrite insert_insert insert_commute //=.
+            rewrite (insert_commute _ PC) //= insert_insert.
+            iFrame "Hmap". }
+          auto.
+          auto.
       }
+      (* Non-capability cases *)
 
-      all: iNext ; iIntros "_".
-      all: iExtract "Hmap" PC as "HPC".
+      all: iNext; iIntros "_".
+      all: iDestruct ((big_sepM_delete _ _ PC) with "Hmap") as "[HPC Hmap] /=";
+        [apply lookup_insert|]; simpl.
       all: rewrite /updatePcPerm; iApply (wp_bind (fill [SeqCtx]));
         iApply (wp_notCorrectPC with "HPC"); [intros HFalse; inversion HFalse| ].
       all: repeat iNext; iIntros "HPC /=".
       all: iApply wp_pure_step_later; auto.
       all: iNext; iIntros "_".
-      all: iApply wp_value;iIntros; discriminate.
-
-    - (* Success IE false *)
-      apply incrementPC_Some_inv in HincrPC as (p''&b''&e''&a''& ? & HPC & Z & Hregs') .
-      rewrite insert_insert in Hregs'; subst regs'.
-      simplify_map_eq.
-
-      match goal with
-      | H: _ |- context [(if (decide ?cond) then _ else _)] =>
-          destruct_decide (decide cond) as Heq
-      end; simplify_eq.
-      { (* contradiction *)
-        exfalso.
-        destruct Heq as (_ & Hnz) ; simplify_eq.
-        apply Hnz in HVsrc.
-        rewrite HVsrc in Hcond; congruence.
-      }
-      iModIntro.
-      iDestruct "HJmpMem" as "->"; simplify_eq. rewrite -memMap_resource_1.
-      iMod ("Hcls" with "[Hmem HP]") as "_";[iExists w;iFrame|iModIntro].
-      iApply wp_pure_step_later; auto.
-
-      set (regs' := <[PC:=WCap p'' b'' e'' x]> (<[idc:=widc]> regs)).
-      simplify_map_eq.
-
-      iNext ; iIntros "_".
-      iApply ("IH" $! regs' p'' with "[%] [] [Hmap] [$Hown]"); subst regs'.
-      { intro; cbn; by repeat (rewrite lookup_insert_is_Some'; right). }
-      { iIntros (ri v Hri Hri' Hvs).
-        simplify_map_eq.
-        iApply "Hreg"; auto.
-      }
-      { rewrite
-          insert_insert
-            (insert_commute _ idc) //=
-            insert_insert.
-        iFrame.
-      }
-      { iModIntro.
-        iClear "HJmpRes IH Hread".
-        rewrite !fixpoint_interp1_eq //=; destruct Hp as [-> | ->] ;iFrame "Hinv_pc".
-      }
-      { iFrame "Hinv_idc". }
+      all: iApply wp_value.
+      all: iIntros.
+      all: discriminate.
+    }
   Qed.
 
 End fundamental.
