theories/rules.v
@@ -3,7 +3,7 @@
 From cap_machine.rules Require Export
      rules_Get rules_Load rules_Store rules_AddSubLt
      rules_Lea rules_Mov rules_Restrict
-     rules_Jmp rules_Jnz rules_Subseg
+     rules_Jmp rules_JmpIEpair rules_Jnz rules_Subseg
      rules_Seal rules_UnSeal.
 
 (* Program specifications
